sepcomp/mem_interpolants.v
@@ -54,4 +54,38 @@ Parameter interpolate_II: forall m1 m2 j12 (MInj12 : Mem.inject j12 m1 m2) m1' (
                              Mem.unchanged_on (loc_unmapped j23) m2 m2' /\ 
                              Mem.unchanged_on (loc_out_of_reach j23 m2) m3 m3'.                                 
 
+
+(*prooves the claim of interpolate_II, plus properties on j12' and j23'
+  corresponding to mkInjections_3 and mkInjections_4. This is usefule for
+  proving Forward_simulations_trans.initial_inject_split in the sufficiently
+  strong form needed to prove that memninj_preserves splits, as required for
+  transitivity_II.*)
+Parameter interpolate_II_HeqMKI: forall m1 m2 j12 (MInj12 : Mem.inject j12 m1 m2) m1'
+                  (Fwd1: mem_forward m1 m1') j23 m3
+                  (MInj23 : Mem.inject j23 m2 m3) m3' (Fwd3: mem_forward m3 m3')
+                  j' (MInj13': Mem.inject j' m1' m3')
+                  (InjIncr: inject_incr (compose_meminj j12 j23) j')
+                  (InjSep: inject_separated (compose_meminj j12 j23) j' m1 m3)
+                  (Unch11': Mem.unchanged_on 
+                            (loc_unmapped (compose_meminj j12 j23)) m1 m1')
+                  (Unch33': Mem.unchanged_on
+                        (loc_out_of_reach (compose_meminj j12 j23) m1) m3 m3'),
+         exists m2', exists j12', exists j23', j'=compose_meminj j12' j23' /\
+                   inject_incr j12 j12' /\ inject_incr j23 j23' /\
+                   Mem.inject j12' m1' m2' /\ mem_forward m2 m2' /\ 
+                   Mem.inject j23' m2' m3' /\
+                   Mem.unchanged_on (loc_out_of_reach j12 m1) m2 m2' /\
+                   inject_separated j12 j12' m1 m2 /\ 
+                   inject_separated j23 j23' m2 m3 /\
+                   Mem.unchanged_on (loc_unmapped j23) m2 m2' /\ 
+                   Mem.unchanged_on (loc_out_of_reach j23 m2) m3 m3' /\
+                   (forall b1 b2 ofs2, j12' b1 = Some(b2,ofs2) -> 
+                     (j12 b1 = Some (b2,ofs2)) \/
+                     (b1 = Mem.nextblock m1 /\ b2 = Mem.nextblock m2 /\ ofs2 = 0) \/ 
+                     (exists m, (b1 = Mem.nextblock m1 + m /\ b2=Mem.nextblock m2 + m)%positive /\ ofs2=0)) /\
+                   (forall b2 b3 ofs3, j23' b2 = Some(b3,ofs3) -> 
+                     (j23 b2 = Some (b3,ofs3)) \/
+                     (b2 = Mem.nextblock m2 /\ j' (Mem.nextblock m1) = Some(b3,ofs3)) \/
+                     (exists m, (b2 = Mem.nextblock m2 + m)%positive /\ 
+                            j' ((Mem.nextblock m1+m)%positive) = Some(b3,ofs3))).
 End MemoryInterpolationAxioms.
